theories/Simulations/Soundness/ImplicitSound.v
@@ -3,31 +3,27 @@ From RSL Require Import Prelude.
 From Stdlib Require Import Classical.
 From Coinduction Require Import all.
 
-From RSL Require Import Simulation.Behaviors.
-From RSL Require Import Simulation.Sim.
+From RSL Require Import Simulations.Behaviors.
+From RSL Require Import Simulations.ImplicitSim.
 
 (* Set Mangle Names. *)
 
-Section SimSound.
+Section ISimSound.
   Context {Λₜ Λₛ: lang}.
   Context (Pₜ: prog Λₜ) (Pₛ: prog Λₛ).
 
   Instance behₜ_elem : ElemOf behavior (state Λₜ) := beh Pₜ.
   Instance behₛ_elem : ElemOf behavior (state Λₛ) := beh Pₛ.
 
-  Inductive behavior_order Φ : @behavior Λₜ -> @behavior Λₛ -> Prop :=
-  | TerminatingOrder : ∀ (vₜ: value Λₜ) (vₛ: value Λₛ),
-    Φ vₜ vₛ -> behavior_order Φ (Terminating vₜ) (Terminating vₛ)
-  | DivergingOrder : behavior_order Φ Diverging Diverging
-  | UnknownOrder : ∀ s, behavior_order Φ s Unknown.
-
   Notation "a '⊑{' Φ '}' b" :=
     (behavior_order Φ a b)
       (at level 70, format "a  '⊑{' Φ '}'  b", no associativity).
 
-  Notation "t '≲' s '{{' Φ '}}'" := (gfp (sim_lfp Pₜ Pₛ Φ) t s).
+  Notation "t '≲' s '{{' Φ '}}'" :=
+    (isim Pₜ Pₛ Φ t s)
+      (at level 70, no associativity).
 
-  Lemma terminating_sim Φ : ∀ t s vₜ,
+  Lemma terminating_isim Φ : ∀ t s vₜ,
     t ≲ s {{ Φ }} ->
     Terminating vₜ ∈ t ->
     ∃ b, b ∈ s ∧ Terminating vₜ ⊑{Φ} b.
@@ -39,7 +35,7 @@ Section SimSound.
     (* Induction on the reduction *)
     induction Hrtc as [ t | t u t' Ht Hrtc IHt ]; intros s Hsim.
     - (* t is final *)
-      apply sim_unroll in Hsim.
+      apply isim_unroll in Hsim.
       induction Hsim as [ t s Hfinal
                         | t s Hstuck
                         | t s s' Hs _ IHs
@@ -50,15 +46,17 @@ Section SimSound.
         (* s is final too *)
         inv Ht. exists (Terminating vₛ). now do 2 constructor.
       + (* Source Stuck *)
-        exists Unknown. split; now constructor.
-      + (* Target Stutter, use IH on s *)
+        exists Undef. split; now constructor.
+      + (* Source Steps, use IH on s *)
         destruct (IHs Hfin) as (b & Hbeh & Horder).
         exists b. split; auto.
         eapply IsSteping; now eauto.
-      + (* Source Stutter -> contradiction *) mixin.
-      + (* Both Steps -> contradiction *) mixin.
+      + (* Target Steps -> contradiction *)
+        mixin.
+      + (* Both Steps -> contradiction *)
+        mixin.
     - (* t steps *)
-      apply sim_unroll in Hsim.
+      apply isim_unroll in Hsim.
       induction Hsim as [ t s Hfinal
                         | t s Hstuck
                         | t s s' Hs _ IHs
@@ -67,14 +65,14 @@ Section SimSound.
       + (* Both Final -> contradiction *)
         destruct Hfinal as (? & ? & ? & ? & ?). mixin.
       + (* Source Stuck *)
-        exists Unknown. split; now constructor.
-      + (* Target Stutter, use IH on s *)
+        exists Undef. split; now constructor.
+      + (* Source Steps, use IH on s *)
         destruct (IHs Ht) as (b & Hbeh & Horder).
         exists b. split; auto.
         eapply IsSteping; now eauto.
-      + (* Source Stutter, use IH on t *)
-        apply IHt; auto. apply sim_roll. auto.
-      + (* Both Steps, use IH on t*)
+      + (* Target Steps, use IH on t *)
+        apply IHt; auto. apply isim_roll. auto.
+      + (* Both Steps, use IH on t *)
         destruct (Hgfp _ Ht) as (s' & Hs & Hsim).
         apply IHt in Hsim; auto.
         destruct Hsim as (b & Hbeh & ?).
@@ -82,18 +80,15 @@ Section SimSound.
         eapply IsSteping; eauto.
   Qed.
 
-  Lemma sim_lfp_progress Φ : ∀ t s,
+  Lemma isim_lfp_progress Φ : ∀ t s,
     t ≲ s {{ Φ }} ->
     diverges Pₜ t ->
     stuck Pₛ s ∨
-      ∃ s', Pₛ ⊨ s ->> s' ∧
-            (
-              (∃ t', t' ≲ s' {{ Φ }} ∧ diverges Pₜ t') ∨
-                (t ≲ s' {{ Φ }} ∧ diverges Pₜ t)
-            ).
+      ∃ t' s', Pₛ ⊨ s ->> s' ∧ t' ≲ s' {{ Φ }} ∧ diverges Pₜ t'.
   Proof.
     intros t s Hsim Hdiv.
-    apply sim_unroll in Hsim.
+    (* Induction on the least-fixpoint of the relation *)
+    apply isim_unroll in Hsim.
     induction Hsim as [ t s Hfin
                       | t s Hstuck
                       | t s s' Hstep Hsim' IH
@@ -105,27 +100,24 @@ Section SimSound.
       mixin.
     - (* SourceStuck *)
       left. exact Hstuck.
-    - (* TargetStutter *)
-      apply sim_roll in Hsim'.
-      right. exists s'. split; now auto.
-    - (* TargetSteps *)
-      (* t can progress, target waits. Because t diverges, it steps to t' *)
+    - (* Source Steps *)
+      apply isim_roll in Hsim'.
+      right. exists t, s'. split; now auto.
+    - (* Target Steps *)
+      (* t can progress, source waits. Because t diverges, it steps to t' *)
       apply diverges_unroll in Hdiv. destruct Hdiv as (t' & Ht_step & Hdiv_t').
       (* Apply the IH for t' *)
       destruct (IH t' Ht_step Hdiv_t') as
-        [Hstuck | (s' & Hstep & [(? & ? & ?) | []])].
+        [Hstuck | (u & s' & Hstep & Hsim & Hdiv')].
       + now left.
-      + right. eexists. split; eauto.
-      + right. eexists. split; eauto.
-
-    - (* BothSteps *)
+      + right. repeat econstructor. all: now eauto.
+    - (* Both Steps *)
       apply diverges_unroll in Hdiv. destruct Hdiv as (t' & Ht_step & Hdiv_t').
       destruct (Hsteps t' Ht_step) as (s' & Hs_step & Hsim_next).
-      right. exists s'. split; auto.
-      left. exists t'. split; auto.
+      right. exists t', s'. split; auto.
   Qed.
 
-  Lemma diverging_sim Φ : ∀ t s,
+  Lemma diverging_isim Φ : ∀ t s,
     t ≲ s {{ Φ }} ->
     Diverging ∈ t ->
     ∃ b, b ∈ s ∧ Diverging ⊑{Φ} b.
@@ -133,19 +125,19 @@ Section SimSound.
     intros t s Hsim Hdiv.
     (* We see in the future: can s be stuck ? *)
     destruct (classic (∃ s', Pₛ ⊨ s ->>* s' ∧ stuck Pₛ s')) as [Hstuck | Hnstuck].
-    - (* s can be stuck -> s has Unknown behavior *)
-      exists Unknown. split; now apply has_stuck_behavior || constructor.
+    - (* s can be stuck -> s has Undef behavior *)
+      exists Undef. split; now apply has_undef_behavior || constructor.
     - (* s is never stuck -> s is diverging *)
       exists Diverging. split; try constructor.
       apply has_diverging_behavior in Hdiv.
-      assert (H: sim _ _ _ _ _) by exact Hsim. clear Hsim.
+      assert (H: isim _ _ _ _ _) by exact Hsim. clear Hsim.
       (* We prove by coinduction that s diverges *)
       unfold diverges.
       revert t s Hdiv H Hnstuck. coinduction R cih.
       intros t s Hdiv Hsim Hnstuck.
       (* [sim_lfp_progress] give us s' such that s ->> s' *)
-      destruct (sim_lfp_progress _ _ _ Hsim Hdiv) as
-        [Hstuck | (s' & Hstep & [(t' & ? & ?) | []])].
+      destruct (isim_lfp_progress _ _ _ Hsim Hdiv) as
+        [Hstuck | (t' & s' & Hstep & Hsim' & Hdiv')].
       + (* s is stuck -> contradiction *)
         exfalso. apply Hnstuck. exists s. split; auto.
       + (* s steps and t too *)
@@ -153,26 +145,21 @@ Section SimSound.
         intros (s'' & ? & ? ).
         apply Hnstuck. exists s''. split; auto.
         econstructor; now eauto.
-      + (* Only s steps *)
-        exists s'. split; auto. apply cih with t; auto.
-        intros (s'' & ? & ? ).
-        apply Hnstuck. exists s''. split; auto.
-        econstructor; now eauto.
   Qed.
 
-  Lemma stuck_sim Φ : ∀ t s,
+  Lemma undef_isim Φ : ∀ t s,
     t ≲ s {{ Φ }} ->
-    Unknown ∈ t ->
-    Unknown ∈ s.
+    Undef ∈ t ->
+    Undef ∈ s.
   Proof.
     intros t s Hsim Hb.
     (* t reach a stuck state. *)
-    apply has_stuck_behavior in Hb. destruct Hb as (t' & Hrtc & Hstuck).
+    apply has_undef_behavior in Hb. destruct Hb as (t' & Hrtc & Hstuck).
     revert s Hsim.
     (* Induction on the reduction *)
     induction Hrtc as [ t | t u t' Ht Hrtc IHt ]; intros s Hsim.
     - (* t = t' *)
-      apply sim_unroll in Hsim.
+      apply isim_unroll in Hsim.
       induction Hsim as [ t s Hfinal
                         | t s ?
                         | t s s' Hs _ IHs
@@ -189,7 +176,7 @@ Section SimSound.
       + (* Source Stutter -> contradiction *) mixin.
       + (* Both Steps -> contradiction *) mixin.
     - (* t steps *)
-      apply sim_unroll in Hsim.
+      apply isim_unroll in Hsim.
       induction Hsim as [ t s Hfinal
                         | t s ?
                         | t s s' Hs _ IHs
@@ -203,30 +190,21 @@ Section SimSound.
         eapply IsSteping; eauto.
         now apply IHs.
       + (* Source Stutter, use IH on t *)
-        apply IHt; auto. apply sim_roll. auto.
+        apply IHt; auto. apply isim_roll. auto.
       + (* Both Steps, use IH on t *)
         destruct (Hgfp _ Ht) as (s' & Hs & Hsim).
         apply IHt in Hsim; auto.
         eapply IsSteping; now eauto.
   Qed.
 
-  (* A definition of state refinement: *)
-  (*    - if the target terminates on (v, m), *)
-  (*    the source must either terminate on (v, m) or be stuck. *)
-  (*    - if the target diverges, *)
-  (*    the source must either diverges or be stuck. *)
-  (*    - if the target is stuck, the source should also be stuck. *)
-  Definition refines Φ (t: state Λₜ) (s: state Λₛ) :=
-    ∀ b, b ∈ t -> ∃ b', b' ∈ s ∧ b ⊑{Φ} b'.
-
-  Theorem sim_sound Φ : ∀ t s,
-    t ≲ s {{ Φ }} -> refines Φ t s.
+  Theorem isim_sound Φ : ∀ t s,
+    t ≲ s {{ Φ }} -> refines Pₜ Pₛ Φ t s.
   Proof.
     intros t s Hsim [] Hb.
-    - now apply terminating_sim with t.
-    - now apply diverging_sim with t.
-    - exists Unknown. split.
-      + now apply stuck_sim with (t := t) (Φ := Φ).
+    - now apply terminating_isim with t.
+    - now apply diverging_isim with t.
+    - exists Undef. split.
+      + now apply undef_isim with (t := t) (Φ := Φ).
       + now constructor.
   Qed.
-End SimSound.
+End ISimSound.
