theories/Commons/OrdTree.v
@@ -1,0 +1,47 @@
+From RSL Require Import Prelude.
+
+From Stdlib Require Import Classical.
+From Stdlib Require Import ClassicalChoice.
+
+Section Def.
+  Context (A: Type).
+
+  Inductive ord_tree: Type :=
+  | ord_tree_base
+  | ord_tree_cons (childs: A -> ord_tree).
+
+  Variant ord_tree_lt: ord_tree -> ord_tree -> Prop :=
+  | ord_tree_lt_intro childs a : ord_tree_lt (childs a) (ord_tree_cons childs).
+
+  Lemma ord_tree_wf : well_founded ord_tree_lt.
+  Proof using.
+    intro x.
+    induction x as [| childs IH];
+      constructor; intros y Hlt; now inv Hlt.
+  Qed.
+
+  Program Canonical Structure WfOrdTree : WfRel :=
+    {| element := ord_tree; lt := tc ord_tree_lt |}.
+  Next Obligation.
+    apply Inclusion.wf_incl with (Relation_Operators.clos_trans _ ord_tree_lt).
+    - intros x y H. induction H as [ | ? ? ? H Ht IH ].
+      + now constructor.
+      + econstructor 2; try eassumption.
+        now constructor.
+    - apply Transitive_Closure.wf_clos_trans.
+      apply ord_tree_wf.
+  Qed.
+
+  Lemma ord_tree_join (P: A -> Prop) (R: A -> ord_tree -> Prop)
+    (ORD: ∀ a, P a -> ∃ o, R a o) :
+    ∃ o, ∀ a, P a -> ∃ o', R a o' ∧ o' ⊏ o.
+  Proof.
+    assert (Hchoice: ∀ a, ∃ o, P a -> R a o).
+    { intro a. destruct (classic (P a)).
+      - destruct (ORD a H) as [o Ho]. exists o. intro. exact Ho.
+      - exists ord_tree_base. intro Hcontra. contradiction. }
+    apply choice in Hchoice. destruct Hchoice as [f Hf].
+    exists (ord_tree_cons f). intros a Ha.
+    exists (f a). split. apply Hf, Ha. now constructor.
+  Qed.
+End Def.
