theories/Prelude.v
@@ -4,3 +4,4 @@ From RSL Require Export Prelude.Definitions.
 From RSL Require Export Prelude.Language.
 From RSL Require Export Prelude.Utils.
 From RSL Require Export Prelude.NoDup.
+From RSL Require Export Prelude.WfRel.
