theories/Prelude/WfRel.v
@@ -1,0 +1,167 @@
+From stdpp Require Import prelude.
+
+From Stdlib Require Import Relation_Operators.
+
+From Stdlib Require Import Wellfounded.Wellfounded.
+From Stdlib Require Import Arith.Wf_nat.
+
+Record WfRel : Type :=
+  wf_rel
+    {
+      element: Type;
+      lt: relation element;
+      wf: well_founded lt;
+      trans: Transitive lt;
+    }.
+
+Coercion element : WfRel >-> Sortclass.
+
+Arguments lt {_} _ _.
+Arguments wf {_} _.
+
+Definition le {W: WfRel} : relation W := clos_refl _ lt.
+
+Notation "x ⊏ y" := (lt x y) (at level 70).
+Notation "x ⊑ y" := (le x y) (at level 70).
+
+Global Instance lt_trans {W: WfRel} : Transitive (@lt W).
+Proof. apply trans. Qed.
+
+Global Instance lt_irrel {W: WfRel} : Irreflexive (@lt W).
+Proof.
+  intros x H.
+  induction x as [x IH] using (well_founded_induction wf).
+  now apply IH with x.
+Qed.
+
+Global Instance lt_strict_order {W: WfRel} : StrictOrder (@lt W)
+  := Build_StrictOrder _ _ _.
+
+Global Instance le_refl {W: WfRel} : Reflexive (@le W).
+Proof. now constructor. Qed.
+
+Global Instance le_trans {W: WfRel} : Transitive (@le W).
+Proof.
+  intros x y z Hxy Hyz. inv Hxy; inv Hyz; try now constructor.
+  constructor; now transitivity y.
+Qed.
+
+Global Instance le_pre_order {W: WfRel} : PreOrder (@le W)
+  := Build_PreOrder _ _ _.
+
+Canonical Structure WfNat: WfRel := {| wf := lt_wf |}.
+
+(* Global Definition WfOrdTree {A: Type} : WfRel := *)
+(*   {| lt := ord_tree_lt A; wf := ord_tree_wf A |}. *)
+
+Section BoolWfRel.
+  Variant bool_lt: relation bool :=
+  | BoolLt : bool_lt false true.
+
+  Local Lemma bool_lt_wf : well_founded bool_lt.
+  Proof.
+    intros []; constructor; intros [] H; inv H.
+    constructor; intros [] H; inv H.
+  Qed.
+
+  Local Lemma bool_lt_trans : Transitive bool_lt.
+  Proof. intros x y z Hxy Hyz. inv Hxy. inv Hyz. Qed.
+
+  Canonical Structure WfBool: WfRel :=
+    {| wf := bool_lt_wf; trans := bool_lt_trans |}.
+End BoolWfRel.
+
+Section WithTopWfRel.
+  Context (W: WfRel).
+
+  Variant lt_top : relation (option W) :=
+  | LtTopSomeSome : ∀ x y, x ⊏ y -> lt_top (Some x) (Some y)
+  | LtTopSomeNone : ∀ x, lt_top (Some x) None.
+
+  Local Lemma lt_top_wf : well_founded lt_top.
+  Proof using.
+    assert (H: ∀ e, Acc lt_top (Some e)).
+    { induction e as [e IH] using (well_founded_induction wf).
+      constructor.
+      intros [] Hlt; inv Hlt.
+      now apply IH.
+    }
+    intros [].
+    - apply H.
+    - constructor. intros [] Hlt; inv Hlt.
+      apply H.
+  Qed.
+
+  Local Lemma lt_top_trans : Transitive lt_top.
+  Proof using.
+    intros x y z Hxy Hyz. inv Hxy; inv Hyz; constructor.
+    etransitivity; eassumption.
+  Qed.
+
+  Definition WfWithTop : WfRel
+    := {| wf := lt_top_wf; trans := lt_top_trans |}.
+End WithTopWfRel.
+
+Section WithBotWfRel.
+  Context (W: WfRel).
+
+  Variant lt_bot : relation (option W) :=
+  | LtBotSomeSome : ∀ x y, x ⊏ y -> lt_bot (Some x) (Some y)
+  | LtBotNoneSome : ∀ x, lt_bot None (Some x).
+
+  Local Lemma lt_bot_wf : well_founded lt_bot.
+  Proof using.
+    intros [].
+    - induction e as [e IH] using (well_founded_induction wf).
+      constructor.
+      intros [] Hlt; inv Hlt.
+      + now apply IH.
+      + constructor. intros [] H; inv H.
+    - constructor. intros [] Hlt; inv Hlt.
+  Qed.
+
+  Local Lemma lt_bot_trans : Transitive lt_bot.
+  Proof using.
+    intros x y z Hxy Hyz. inv Hxy; inv Hyz; constructor.
+    etransitivity; eassumption.
+  Qed.
+
+  Definition WfWithBot : WfRel
+    := {| wf := lt_bot_wf; trans := lt_bot_trans |}.
+End WithBotWfRel.
+
+Section LexProdWfRel.
+  Context (W1 W2: WfRel).
+
+  Local Lemma slexprod_trans : Transitive (slexprod W1 W2 lt lt).
+  Proof using.
+    intros x y z Hxy Hyz.
+    inv Hxy; inv Hyz.
+    - left. etransitivity; eassumption.
+    - left. eassumption.
+    - left. eassumption.
+    - right. etransitivity; eassumption.
+  Qed.
+
+  Canonical Structure WfLexProd : WfRel :=
+    {|
+      wf := wf_slexprod _ _ _ _ wf wf;
+      trans := slexprod_trans;
+    |}.
+End LexProdWfRel.
+
+Section UnionWfRel.
+  Context (W1 W2: WfRel).
+
+  Local Lemma le_AsB_trans : Transitive (le_AsB W1 W2 lt lt).
+  Proof using.
+    intros x y z Hxy Hyz.
+    inv Hxy; inv Hyz; constructor; etransitivity; eassumption.
+  Qed.
+
+  Canonical Structure WfUnion : WfRel :=
+    {|
+      wf := wf_disjoint_sum  _ _ _ _ wf wf;
+      trans := le_AsB_trans;
+    |}.
+End UnionWfRel.
