theories/Simulations/Commons.v
@@ -1,0 +1,12 @@
+From RSL Require Import Prelude.
+
+(* Set Mangle Names. *)
+
+Section CommonsDef.
+  Context {Λₜ Λₛ: lang}.
+  Context (Φ: value Λₜ -> value Λₛ -> Prop).
+
+  Definition is_final (t: state Λₜ) (s: state Λₛ) : Prop :=
+    ∃ vₜ vₛ, is_final t = Some vₜ ∧ is_final s = Some vₛ ∧ Φ vₜ vₛ.
+
+End CommonsDef.
