theories/Simulations/Equiv/EAltSim.v
@@ -1,0 +1,140 @@
+From RSL Require Import Prelude.
+
+From Coinduction Require Import all.
+
+From RSL Require Import Simulations.Commons.
+
+Section EAltSimDef.
+  Context {Λₜ Λₛ: lang}.
+  Context (Wₜ Wₛ: WfRel).
+  Context (Pₜ: prog Λₜ) (Pₛ: prog Λₛ) (Φ: value Λₜ -> value Λₛ -> Prop).
+
+  Variant ealt_sim_lfp' (gfp: Wₜ -> state Λₜ -> Wₛ -> state Λₛ -> Prop)
+    : Wₜ -> state Λₜ -> Wₛ -> state Λₛ -> Prop :=
+  | EAltBothFinal : ∀ wₜ t wₛ s,
+    is_final Φ t s -> ealt_sim_lfp' gfp wₜ t wₛ s
+
+  | EAltSourceStuck : ∀ wₜ t wₛ s,
+    stuck Pₛ s -> ealt_sim_lfp' gfp wₜ t wₛ s
+
+  | EAltSourceSteps : ∀ wₜ wₜ' t wₛ wₛ' s s',
+    Pₛ ⊨ s ->> s' ->
+    wₛ' ⊏ wₛ ->
+    gfp  wₜ' t wₛ' s' ->
+    ealt_sim_lfp' gfp wₜ t wₛ s
+
+  | EAltTargetSteps : ∀ wₜ t wₛ s,
+    can_progress Pₜ t ->
+    (∀ t', Pₜ ⊨ t ->> t' ->
+           ∃ wₜ' wₛ',
+             wₜ' ⊏ wₜ ∧
+             gfp wₜ' t' wₛ' s) ->
+    ealt_sim_lfp' gfp wₜ t wₛ s
+
+  | EAltBothSteps : ∀ wₜ t wₛ s,
+    can_progress Pₜ t ->
+    (∀ t', Pₜ ⊨ t ->> t' ->
+           ∃ wₜ' wₛ' s' ,
+             Pₛ ⊨ s ->> s' ∧
+             gfp wₜ' t' wₛ' s') ->
+    ealt_sim_lfp' gfp wₜ t wₛ s.
+
+  Instance ealt_sim_mono : Proper (leq ==> leq) ealt_sim_lfp'.
+    intros gfp gfp' Hgfp  wₜ t  wₛ s Hsim.
+    inv Hsim.
+    - econstructor; eassumption.
+    - econstructor; eassumption.
+    - eapply EAltSourceSteps; eauto.
+      apply Hgfp. eassumption.
+    - apply EAltTargetSteps; auto. intros ? Hstep.
+      edestruct (H0 _ Hstep) as (wₜ' & wₛ' & HR & Isim).
+      do 2 eexists. split; eauto.
+      apply Hgfp. eassumption.
+    - apply EAltBothSteps; auto. intros ? Hstep.
+      edestruct (H0 _ Hstep) as (wₜ' & wₛ' & s' & HR & Isim).
+      do 3 eexists. split; eauto.
+      apply Hgfp. eassumption.
+  Qed.
+
+  Definition ealt_sim_lfp : mon (Wₜ -> state Λₜ -> Wₛ -> state Λₛ -> Prop) :=
+    {| body := ealt_sim_lfp' |}.
+
+  Lemma ealt_sim_unroll wₜ t wₛ s :
+    gfp ealt_sim_lfp wₜ t wₛ s -> ealt_sim_lfp' (gfp ealt_sim_lfp) wₜ t wₛ s.
+  Proof using. apply (gfp_fp ealt_sim_lfp). Qed.
+
+  Lemma ealt_sim_roll wₜ t wₛ s :
+    ealt_sim_lfp' (gfp ealt_sim_lfp) wₜ t wₛ s -> gfp ealt_sim_lfp wₜ t wₛ s.
+  Proof using. apply (gfp_fp ealt_sim_lfp). Qed.
+
+  Definition ealt_sim : Wₜ -> state Λₜ -> Wₛ -> state Λₛ -> Prop
+    := gfp ealt_sim_lfp.
+
+  Lemma test (R: Chain ealt_sim_lfp):
+    ∀ iₜ t iₛ s,
+    (elem R) iₜ t iₛ s ->
+    ∀ iₜ' iₛ',
+    iₜ ⊑ iₜ' ->
+    iₛ ⊑ iₛ' ->
+    (elem R) iₜ' t iₛ' s.
+  Proof.
+    apply tower.
+    - unfold inf_closed.
+      intros P Hp.
+      intros iₜ t iₛ s Hinf iₜ' iₛ' Ht Hs.
+      intros Q Hq.
+      eapply (Hp _ Hq).
+      + now apply Hinf.
+      + assumption.
+      + assumption.
+    - clear R. intros R CIH iₜ t iₛ s H.
+      induction H; intros iₜ' iₛ' Ht Hs.
+      + now constructor.
+      + now constructor.
+      + inv Hs as [ ? Hs' | ].
+        * eapply EAltSourceSteps.
+          { eassumption. }
+          { eassumption. }
+          eapply CIH.
+          eassumption.
+          reflexivity.
+          now left.
+        * eapply EAltSourceSteps.
+          { eassumption. }
+          { eassumption. }
+          eapply CIH.
+          eassumption.
+          reflexivity.
+          reflexivity.
+      + inv Ht as [ ? Ht' | ].
+        * apply EAltTargetSteps.
+          { eassumption. }
+          intros t' Hstep.
+          destruct (H0 _ Hstep) as (? & ? & ? & ?).
+          do 2 eexists.
+          split.
+          eassumption.
+          eapply CIH.
+          eassumption.
+          now left.
+          reflexivity.
+        * apply EAltTargetSteps.
+          { eassumption. }
+          intros t' Hstep.
+          destruct (H0 _ Hstep) as (? & ? & ? & ?).
+          do 2 eexists.
+          split.
+          eassumption.
+          eapply CIH.
+          eassumption.
+          reflexivity.
+          reflexivity.
+      + apply EAltBothSteps.
+        { assumption. }
+        intros t' Hstep.
+        edestruct H0 as (? & ? & ? & ? & ?). eassumption.
+        do 3 eexists. split.
+        eassumption.
+        eassumption.
+  Qed.
+End EAltSimDef.
