theories/Simulations/Equiv/EAltSimToESimLax.v
@@ -1,0 +1,92 @@
+From RSL Require Import Prelude.
+
+From Coinduction Require Import all.
+
+From RSL Require Import Simulations.Commons.
+From RSL Require Import Simulations.Equiv.ExplicitSimLax.
+From RSL Require Import Simulations.Equiv.EAltSim.
+
+Section PROOF.
+  Context {Λₜ Λₛ: lang}.
+  Context (Wₜ Wₛ: WfRel).
+  Context (Pₜ: prog Λₜ) (Pₛ: prog Λₛ) (Φ: value Λₜ -> value Λₛ -> Prop).
+
+  Lemma ealt_sim_implies_esim_lax: ∀ wₜ t wₛ s,
+    ealt_sim Wₜ Wₛ Pₜ Pₛ Φ wₜ t wₛ s ->
+    ∃ W i, esim_lax W Pₜ Pₛ Φ i t s.
+  Proof.
+    intros wₜ t wₛ s Hsim.
+    exists (WfWithBot (WfLexProd Wₜ Wₛ)), (Some (wₜ, wₛ)).
+    revert wₜ t wₛ s Hsim.
+    unfold esim_lax.
+    coinduction R cih.
+    intros wₜ t wₛ s Hsim.
+    apply ealt_sim_unroll in Hsim.
+    induction Hsim as [ wₜ t wₛ s Hfinal
+                      | wₜ t wₛ s Hstuck
+                      | wₜ wₜ' t wₛ wₛ' s s' Hstep Hlt Hsim
+                      | wₜ t wₛ s Hprogress Ht
+                      | wₜ t wₛ s Hprogress Hboth].
+    - now constructor.
+    - now constructor.
+    - assert (Hrtc: Pₛ ⊨ s ->>+ s').
+      { econstructor. eassumption. reflexivity. }
+      clear Hstep.
+      revert wₜ' s' Hrtc Hsim.
+      induction wₛ' as [wₛ' IHwₛ'] using (well_founded_ind wf).
+      intros wₜ' s' Hrtc Hsim.
+      apply ealt_sim_unroll in Hsim.
+      inv Hsim.
+      + eapply ELaxSourceSteps.
+        * eassumption.
+        * now constructor.
+        * apply (@b_chain _ _ _ R).
+          now constructor.
+      + eapply ELaxSourceSteps.
+        * eassumption.
+        * now constructor.
+        * apply (@b_chain _ _ _ R).
+          now constructor.
+      + (* EAltSourceSteps *)
+        eapply IHwₛ'.
+        * eassumption.
+        * etransitivity; eassumption.
+        * eapply pstep_r; eassumption.
+        * eassumption.
+      + (* EAltTargetSteps *)
+        (* The target finally stepped. We can emit EBothSteps directly from the original state s *)
+        eapply ELaxBothSteps.
+        * eassumption.
+        * intros t' Htstep.
+          destruct (H0 _ Htstep) as (wₜ'' & wₛ'' & Hlt_wₜ & Hsim_next).
+          exists (Some (wₜ'', wₛ'')), s'.
+          split; try apply cih; eassumption.
+      + (* EAltBothSteps *)
+        eapply ELaxBothSteps.
+        * eassumption.
+        * intros t' Htstep.
+          destruct (H0 _ Htstep) as (wₜ'' & wₛ'' & s'' & Hstep_s'' & Hsim_next).
+          exists (Some (wₜ'', wₛ'')), s''.
+          split.
+          -- eapply pstep_r; eassumption.
+          -- apply cih; eassumption.
+    - apply ELaxTargetSteps.
+      { assumption. }
+      intros t' Hstep.
+      destruct (Ht _ Hstep) as (wₜ' & wₛ' & Hlt & Hgfp).
+      eexists. split.
+      2: {
+        apply cih.
+        eassumption.
+      }
+      constructor. now left.
+    - apply ELaxBothSteps.
+      { assumption. }
+      intros t' Hstep.
+      edestruct (Hboth _ Hstep) as (wₜ' & wₛ' & s' & Hs & Hsim).
+      exists (Some (wₜ', wₛ')), s'.
+      split.
+      + econstructor; eassumption || reflexivity.
+      + apply cih. assumption.
+  Qed.
+End PROOF.
