theories/Simulations/Equiv/ESimLaxToESim.v
@@ -1,0 +1,74 @@
+From RSL Require Import Prelude.
+
+From Coinduction Require Import all.
+
+From RSL Require Import Simulations.Commons.
+From RSL Require Import Simulations.ExplicitSim.
+From RSL Require Import Simulations.Equiv.ExplicitSimLax.
+
+Section PROOF.
+  Context {Λₜ Λₛ: lang}.
+  Context (W: WfRel) (Pₜ: prog Λₜ) (Pₛ: prog Λₛ) (Φ: value Λₜ -> value Λₛ -> Prop).
+
+  Definition Wnew : WfRel := WfLexProd W WfNat.
+
+  Lemma esim_lax_to_esim_inv: ∀ n i t s s',
+    Pₛ ⊨ s -{ n }> s' ->
+    esim_lax W Pₜ Pₛ Φ i t s' ->
+    esim Wnew Pₜ Pₛ Φ (i, n) t s.
+  Proof.
+    unfold esim.
+    coinduction C cih.
+    intros n.
+    induction n as [ | n IH ].
+    - intros i t s s' Hstep Hsim. inv Hstep.
+      apply esim_lax_unroll in Hsim.
+      induction Hsim as
+        [
+        |
+        | ? ? ? s s''
+        |
+        |
+        ].
+      + now constructor.
+      + now constructor.
+      + destruct (pstep_to_nstep_l _ _ H) as (n & s' & Hstep & Hnstep).
+        eapply ESourceSteps.
+        { eassumption. }
+        2:{ eapply cih; eassumption. }
+        now constructor.
+      + apply ETargetSteps.
+        { assumption. }
+        intros t' Hstep.
+        destruct (H0 _ Hstep) as (i' & Hlt & Hsim).
+        exists (i', 0).
+        split.
+        * now constructor.
+        * eapply cih; eassumption || constructor.
+      + apply EBothSteps.
+        { assumption. }
+        intros t' Hstep.
+        destruct (H0 _ Hstep) as (i' & s'' & Hs & Hsim).
+        destruct (pstep_to_nstep_l _ _ Hs) as (n & s' & Hsteps & Hnstep).
+        do 2 eexists. split.
+        * eassumption.
+        * eapply cih; eassumption || constructor.
+    - intros i t s s' Hstep Hsim.
+      inv Hstep as [ | ? ? ? ? Hs Hnstep ].
+      eapply ESourceSteps.
+      { eassumption. }
+      2:{ eapply cih; eassumption. }
+      right. simpl. lia.
+  Qed.
+
+  Lemma esim_lax_implies_esim: ∀ i t s,
+    esim_lax W Pₜ Pₛ Φ i t s ->
+    ∃ (R: WfRel) w, esim R Pₜ Pₛ Φ w t s.
+  Proof.
+    intros i t s Hsim.
+    exists Wnew, (i, 0).
+    apply esim_lax_to_esim_inv with s.
+    - constructor.
+    - assumption.
+  Qed.
+End PROOF.
