theories/Simulations/Equiv/Equiv.v
@@ -1,0 +1,152 @@
+From RSL Require Import Prelude.
+
+From Coinduction Require Import all.
+
+From RSL Require Import Simulations.Commons.
+From RSL Require Import Simulations.ImplicitSim.
+From RSL Require Import Simulations.ExplicitSim.
+From RSL Require Import Simulations.FreeSim.
+
+From RSL Require Import Simulations.Equiv.FSimToGSim.
+From RSL Require Import Simulations.Equiv.GSimToEAltSim.
+From RSL Require Import Simulations.Equiv.EAltSimToESimLax.
+From RSL Require Import Simulations.Equiv.ESimLaxToESim.
+
+(* Set Mangle Names. *)
+
+Section SimEquiv.
+  Context {Λₜ Λₛ: lang}.
+  Context (Pₜ: prog Λₜ) (Pₛ: prog Λₛ).
+
+  Notation "t '≲' s '{{' Φ '}}'" :=
+    (isim Pₜ Pₛ Φ t s)
+      (at level 70, no associativity).
+
+  Notation "t '≲' '[' i ']' s '{{' Φ '}}'" :=
+    (esim _ Pₜ Pₛ Φ i t s)
+      (at level 70, no associativity).
+
+  Notation "t '⟨' iₜ '≲' iₛ '⟩' s '{{' Φ '}}'" :=
+    (fsim _ _ Pₜ Pₛ Φ iₜ t iₛ s)
+      (at level 70, iₜ at level 69, iₛ at level 69, no associativity).
+
+  Lemma isim_to_fsim {Wₜ Wₛ: WfRel} Φ :
+    ∀ t s,
+    t ≲ s {{ Φ }} ->
+    ∀ (iₜ iₜ': Wₜ) (iₛ iₛ': Wₛ),
+    iₜ ⊏ iₜ' ->
+    iₛ ⊏ iₛ' ->
+    t ⟨iₜ ≲ iₛ⟩ s {{ Φ }}.
+  Proof using.
+    unfold fsim.
+    coinduction R cih.
+    intros t s Hsim.
+    apply isim_unroll in Hsim.
+    induction Hsim as [ t s Hfinal
+                      | t s Hstuck
+                      | t s s' Hstep Hs IHs
+                      | t s Hprogress Ht IHt
+                      | t s Hprogress Hboth ];
+      intros iₜ iₜ' iₛ iₛ' HRt HRs.
+    - (* Both Final *)
+      now constructor.
+    - (* Source Stuck *)
+      now constructor.
+    - (* Source Steps *)
+      eapply FSourceSteps.
+      + eassumption.
+      + eapply IHs; eassumption.
+    - (* Target Steps *)
+      apply FTargetSteps.
+      + assumption.
+      + intros t' Hstep. eexists.
+        eapply IHt; eassumption.
+    - (* Both steps *)
+      apply FTargetSteps; try assumption.
+      intros t' Hstep.
+      destruct (Hboth _ Hstep) as (s' & Hstep_s & Hsim).
+      eexists.
+      eapply FSourceSteps; try eassumption.
+      eapply FProgress.
+      { eassumption. }
+      { eassumption. }
+      eapply cih.
+      + apply Hsim.
+      + eassumption.
+      + eassumption.
+  Qed.
+
+  Lemma esim_to_isim {W: WfRel} Φ :
+    ∀ (i: W) t s,
+    t ≲[i] s {{ Φ }} ->
+    t ≲ s {{ Φ }}.
+  Proof using.
+    unfold isim.
+    coinduction ξ cih.
+    intros i.
+    induction i as [i IH] using (well_founded_induction wf).
+    intros t s Hsim.
+    apply esim_unroll in Hsim.
+    induction Hsim as [ ? t s Hfinal
+                      | ? t s Hstuck
+                      | ? i' t s s' Hstep H IHs
+                      | ? t s Hprogress H
+                      | ? t s Hprogress H ].
+    - (* Both Final *)
+      now constructor.
+    - (* Source Stuck *)
+      now constructor.
+    - (* Source Steps *)
+      apply ISourceSteps with s'.
+      { assumption. }
+      now apply IH with i'.
+    - (* Target Steps *)
+      apply ITargetSteps.
+      { assumption. }
+      intros t' Hstep.
+      destruct (H _ Hstep) as (i' & ? & ?).
+      now apply IH with i'.
+    - (* Both steps *)
+      apply IBothSteps.
+      { assumption. }
+      intros t' Hstep.
+      destruct (H _ Hstep) as (i' & s' & Hstep_s & Hsim).
+      exists s'. split; auto.
+      eapply cih.
+      eassumption.
+  Qed.
+
+  Lemma fsim_to_esim {Wₜ Wₛ: WfRel} Φ:
+    ∀ (iₜ: Wₜ) t (iₛ: Wₛ) s,
+    t ⟨iₜ ≲ iₛ⟩ s {{ Φ }} ->
+    ∃ (W: WfRel) (i: W), t ≲[i] s {{ Φ }}.
+  Proof using.
+    intros iₜ t iₛ s Hsim.
+    apply fsim_implies_gsim in Hsim.
+    destruct Hsim as (wₜ & wₛ & Hgsim).
+    apply gsim_implies_ealt_sim in Hgsim.
+    destruct Hgsim as (Rₜ & Rₛ & zₜ & zₛ & Healtsim).
+    apply ealt_sim_implies_esim_lax in Healtsim.
+    destruct Healtsim as (W & i & Hesimlax).
+    apply esim_lax_implies_esim in Hesimlax.
+    destruct Hesimlax as (R & w & Hesim).
+    do 2 eexists. eassumption.
+  Qed.
+
+  Lemma index_irrel {Wₜ Wₛ: WfRel} Φ:
+    ∀ t s,
+    (∃ (iₜ: Wₜ) (iₛ: Wₛ), t ⟨iₜ ≲ iₛ⟩ s {{ Φ }}) ->
+    ∀ iₜ iₛ,
+    (∃ T : Wₜ, iₜ ⊏ T) ->
+    (∃ T : Wₛ, iₛ ⊏ T) ->
+    t ⟨iₜ ≲ iₛ⟩ s {{ Φ }}.
+  Proof using.
+    intros t s (oₜ & oₛ & Hsim) iₜ iₛ (Tₜ & Ht) (Tₛ & Hs).
+    apply fsim_to_esim in Hsim.
+    destruct Hsim as (W & i & Hesim).
+    eapply isim_to_fsim.
+    - eapply esim_to_isim. eassumption.
+    - eassumption.
+    - eassumption.
+  Qed.
+End SimEquiv.
