theories/Simulations/Equiv/FSimToGSim.v
@@ -1,0 +1,90 @@
+From RSL Require Import Prelude.
+
+From Coinduction Require Import all.
+
+From RSL Require Import Commons.OrdTree.
+
+From RSL Require Import Simulations.Commons.
+From RSL Require Import Simulations.FreeSim.
+
+From RSL Require Import Simulations.Equiv.GSim.
+
+Section PROOF.
+  Context {Λₜ Λₛ: lang}.
+  Context (Wₜ Wₛ: WfRel).
+  Context (Pₜ: prog Λₜ) (Pₛ: prog Λₛ) (Φ: value Λₜ -> value Λₛ -> Prop).
+
+  Definition StatePair := (state Λₜ * state Λₛ)%type.
+
+  Lemma fsim_implies_gsim: ∀ iₜ t iₛ s,
+    fsim Wₜ Wₛ Pₜ Pₛ Φ iₜ t iₛ s ->
+    ∃ wₜ wₛ,
+      gsim _ _ (WfOrdTree StatePair) Pₜ Pₛ Φ iₜ wₜ t iₛ wₛ s.
+  Proof.
+    intros iₜ t iₛ s Hsim.
+    apply fsim_unroll in Hsim.
+    induction Hsim as [ iₜ t iₛ s Hfinal
+                      | iₜ t iₛ s Hstuck
+                      | iₜ t iₛ iₛ' s s' Hs ? IHs
+                      | iₜ t iₛ s Hprogress IHt
+                      | iₜ iₜ' t iₛ iₛ' s Hprogress1 Hprogress2 Hasim ].
+    - exists (ord_tree_base StatePair), (ord_tree_base StatePair).
+      apply GBothFinal; eassumption.
+    - exists (ord_tree_base StatePair), (ord_tree_base StatePair).
+      apply GSourceStuck; eassumption.
+    - destruct IHs as (wₜ' & wₛ' & Hinv).
+      exists wₜ', (ord_tree_cons StatePair (fun _ => wₛ')).
+      eapply GSourceSteps.
+      + eassumption.
+      + constructor. apply ord_tree_lt_intro with (a := (t, s')).
+      + eassumption.
+    - pose (P := fun a: StatePair =>
+                   let (t', s') := a in
+                   s' = s ∧ Pₜ ⊨ t ->> t').
+
+      pose (R := fun (a: StatePair) (o: ord_tree StatePair) =>
+                   let (t', s') := a in
+                   s' = s ∧ Pₜ ⊨ t ->> t' ∧
+                   ∃ (iₜ: Wₜ) wₛ,
+                     gsim _ _ _ Pₜ Pₛ Φ iₜ o t' iₛ wₛ s).
+
+      assert (Hord: ∀ a, P a -> ∃ o, R a o).
+      { intros [t' s'] [Heq Hstep]. subst s'.
+        destruct (IHt t' Hstep) as (iₜ' & ? & wₜ' & wₛ' & Hsim').
+        exists wₜ'. split; [reflexivity|]. split; [assumption|].
+        exists iₜ'. exists wₛ'. exact Hsim'. }
+      destruct (ord_tree_join StatePair P R Hord) as [wₜ Hjoin1].
+
+      pose (R2 := fun (a: StatePair) (o: ord_tree StatePair) =>
+                    let (t', s') := a in
+                    s' = s ∧
+                    Pₜ ⊨ t ->> t' ∧
+                    ∃ (iₜ': Wₜ) wₜ',
+                       wₜ' ⊏ wₜ ∧
+                      gsim _ _ _ Pₜ Pₛ Φ iₜ' wₜ' t' iₛ o s).
+      assert (Hord2: ∀ a, P a -> ∃ o, R2 a o).
+      { intros [t' s'] [Heq Hstep]. subst s'.
+        destruct (Hjoin1 (t', s)) as [wₜ' [Hrw Hlt]].
+        { split; [reflexivity|assumption]. }
+        destruct Hrw as (_ & Hstep' & iₜ' & wₛ' & Hsim').
+        exists wₛ'. split; [reflexivity|]. split; [assumption|].
+        exists iₜ'.
+        exists wₜ'. split; [exact Hlt|exact Hsim']. }
+      destruct (ord_tree_join StatePair P R2 Hord2) as [wₛ Hjoin2].
+
+      exists wₜ, wₛ.
+      eapply GTargetSteps.
+      + exact Hprogress.
+      + intros t' Hstep.
+        destruct (Hjoin2 (t', s)) as [wₛ' [Hrw Hlt]].
+        { split; [reflexivity|assumption]. }
+        destruct Hrw as (_ & Hstep' & iₜ' & wₜ' &  Hlt_wₜ & Hsim').
+        exists iₜ'. exists wₜ'. split.
+        * assumption.
+        * apply gsim_weaken_s with wₛ'.
+          { assumption. }
+          now constructor.
+    - exists (ord_tree_base StatePair), (ord_tree_base StatePair).
+      eapply GProgress; eassumption.
+  Qed.
+End PROOF.
