theories/Simulations/Equiv/GSim.v
@@ -1,0 +1,167 @@
+From RSL Require Import Prelude.
+
+From Coinduction Require Import all.
+
+From RSL Require Import Simulations.Commons.
+From RSL Require Import Simulations.FreeSim.
+
+Section GSimDef.
+  Context {Λₜ Λₛ: lang}.
+  Context (Wₜ Wₛ W: WfRel).
+  Context (Pₜ: prog Λₜ) (Pₛ: prog Λₛ) (Φ: value Λₜ -> value Λₛ -> Prop).
+
+  Unset Elimination Schemes.
+
+  Inductive gsim : Wₜ -> W -> state Λₜ -> Wₛ -> W -> state Λₛ -> Prop :=
+  | GBothFinal : ∀ iₜ wₜ t iₛ wₛ s,
+    is_final Φ t s -> gsim iₜ wₜ t iₛ wₛ s
+
+  | GSourceStuck : ∀ iₜ wₜ t iₛ wₛ s,
+    stuck Pₛ s -> gsim iₜ wₜ t iₛ wₛ s
+
+  | GSourceSteps : ∀ iₜ wₜ t iₛ iₛ' wₛ s s' wₛ',
+    Pₛ ⊨ s ->> s' ->
+    wₛ' ⊏ wₛ ->
+    gsim iₜ wₜ t iₛ' wₛ' s' ->
+    gsim iₜ wₜ t iₛ wₛ s
+
+  | GTargetSteps : ∀ iₜ wₜ t iₛ wₛ s,
+    can_progress Pₜ t ->
+    (∀ t', Pₜ ⊨ t ->> t' -> ∃ iₜ' wₜ',
+         wₜ' ⊏ wₜ ∧ gsim iₜ' wₜ' t' iₛ wₛ s) ->
+    gsim iₜ wₜ t iₛ wₛ s
+
+  | GProgress : ∀ iₜ iₜ' wₜ t iₛ iₛ' wₛ s,
+    iₜ' ⊏ iₜ ->
+    iₛ' ⊏ iₛ ->
+    fsim Wₜ Wₛ Pₜ Pₛ Φ iₜ' t iₛ' s ->
+    gsim iₜ wₜ t iₛ wₛ s.
+
+  Set Elimination Schemes.
+
+  Section GSimInd.
+    Variable P : Wₜ -> W -> state Λₜ -> Wₛ -> W -> state Λₛ -> Prop.
+
+    Hypothesis HFinal:
+      ∀ iₜ wₜ t iₛ wₛ s, is_final Φ t s -> P iₜ wₜ t iₛ wₛ s.
+
+    Hypothesis HStuck:
+      ∀ iₜ wₜ t iₛ wₛ s, stuck Pₛ s -> P iₜ wₜ t iₛ wₛ s.
+
+    Hypothesis HSourceSteps:
+      ∀ iₜ wₜ t iₛ iₛ' wₛ s s' wₛ',
+      Pₛ ⊨ s ->> s' ->
+      wₛ' ⊏ wₛ ->
+      gsim iₜ wₜ t iₛ' wₛ' s' ->
+      P iₜ wₜ t iₛ' wₛ' s' ->
+      P iₜ wₜ t iₛ wₛ s.
+
+    Hypothesis HTargetSteps:
+      ∀ iₜ wₜ t iₛ wₛ s,
+      can_progress Pₜ t ->
+      (∀ t', Pₜ ⊨ t ->> t' ->
+             ∃ iₜ' wₜ',
+               wₜ' ⊏ wₜ ∧
+               gsim iₜ' wₜ' t' iₛ wₛ s ∧
+               P iₜ' wₜ' t' iₛ wₛ s) ->
+      P iₜ wₜ t iₛ wₛ s.
+
+    Hypothesis HProgress:
+      ∀ iₜ iₜ' wₜ t iₛ iₛ' wₛ s,
+      iₜ' ⊏ iₜ ->
+      iₛ' ⊏ iₛ ->
+      fsim Wₜ Wₛ Pₜ Pₛ Φ iₜ' t iₛ' s ->
+      P iₜ wₜ t iₛ wₛ s.
+
+    Lemma gsim_ind: ∀ iₜ wₜ t iₛ wₛ s,
+      gsim iₜ wₜ t iₛ wₛ s -> P iₜ wₜ t iₛ wₛ s.
+    Proof.
+      fix IH 7. intros iₜ wₜ t iₛ wₛ s Hsim.
+      destruct Hsim as
+        [ iₜ wₜ t iₛ wₛ s Hfin
+        | iₜ wₜ t iₛ wₛ s Hstuck
+        | iₜ wₜ t iₛ wₛ s s' wₛ' Hstep HR Hsim
+        | iₜ wₜ t iₛ wₛ s Hprogress Ht
+        | iₜ iₜ' wₜ t iₛ iₛ' wₛ s Ht Hs Hgfp ].
+      - apply HFinal. assumption.
+      - apply HStuck. assumption.
+      - eapply HSourceSteps; now eauto.
+      - apply HTargetSteps.
+        { assumption. }
+        intros t' Hstep.
+        destruct (Ht _ Hstep) as (iₜ' & wₜ' & HR & Hsim).
+        do 2 eexists. now eauto.
+      - eapply HProgress; now eauto.
+    Qed.
+  End GSimInd.
+
+  Register Scheme gsim_ind as ind_nodep for gsim.
+
+  Lemma gsim_weaken_t: ∀ iₜ wₜ t iₛ wₛ s,
+    gsim iₜ wₜ t iₛ wₛ s ->
+    ∀ w, wₜ ⊑ w ->
+    gsim iₜ w t iₛ wₛ s.
+  Proof using.
+    intros iₜ wₜ t iₛ wₛ s Hsim w Hle.
+    induction Hsim as
+      [ iₜ wₜ t iₛ wₛ s Hfin
+      | iₜ wₜ t iₛ wₛ s Hstuck
+      | iₜ wₜ t iₛ iₛ' wₛ s s' wₛ' Hstep HR Hsim IHs
+      | iₜ wₜ t iₛ wₛ s Hprogress IHt
+      | iₜ iₜ' wₜ t iₛ iₛ' wₛ s Ht Hs Hgfp]
+      in w, Hle |- *.
+    - now constructor.
+    - now constructor.
+    - eapply GSourceSteps.
+      { eassumption. }
+      { eassumption. }
+      now apply IHs.
+    - apply GTargetSteps.
+      { assumption. }
+      intros t' Hstep.
+      destruct (IHt _ Hstep) as (iₜ' & wₜ' & Hlt' & Hsim & IH).
+      inv Hle as [ ? Hlt | ].
+      + do 2 eexists. split.
+        * eassumption.
+        * apply IH.
+          now left.
+      + do 2 eexists. split; eauto.
+    - eapply GProgress; try eassumption.
+  Qed.
+
+  Lemma gsim_weaken_s: ∀ iₜ wₜ t iₛ wₛ s,
+    gsim iₜ wₜ t iₛ wₛ s ->
+    ∀ w, wₛ ⊑ w ->
+    gsim iₜ wₜ t iₛ w s.
+  Proof using.
+    intros iₜ wₜ t iₛ wₛ s Hsim w Hle.
+    induction Hsim as
+      [ iₜ wₜ t iₛ wₛ s Hfin
+      | iₜ wₜ t iₛ wₛ s Hstuck
+      | iₜ wₜ t iₛ iₛ' wₛ s s' wₛ' Hstep HR Hsim IHs
+      | iₜ wₜ t iₛ wₛ s Hprogress IHt
+      | iₜ iₜ' wₜ t iₛ iₛ' wₛ s Ht Hs Hgfp]
+      in w, Hle |- *.
+    - now constructor.
+    - now constructor.
+    - inv Hle as [ ? Hlt | ].
+      + eapply GSourceSteps.
+        { eassumption. }
+        { eassumption. }
+        apply IHs.
+        now left.
+      + eapply GSourceSteps.
+      { eassumption. }
+      { eassumption. }
+      apply IHs. now right.
+    - apply GTargetSteps.
+      { assumption. }
+      intros t' Hstep.
+      destruct (IHt _ Hstep) as (iₜ' & wₜ' & Hlt' & Hsim & IH).
+      do 2 eexists. split.
+      + eassumption.
+      + apply IH. assumption.
+    - eapply GProgress; try eassumption.
+  Qed.
+
+End GSimDef.
