theories/Simulations/Equiv/GSimToEAltSim.v
@@ -1,0 +1,73 @@
+From RSL Require Import Prelude.
+
+From Coinduction Require Import all.
+
+From RSL Require Import Commons.OrdTree.
+
+From RSL Require Import Simulations.Commons.
+From RSL Require Import Simulations.FreeSim.
+
+From RSL Require Import Simulations.Equiv.GSim.
+From RSL Require Import Simulations.Equiv.EAltSim.
+From RSL Require Import Simulations.Equiv.FSimToGSim.
+
+Section PROOF.
+  Context {Λₜ Λₛ: lang}.
+  Context (Wₜ Wₛ: WfRel).
+  Context (Pₜ: prog Λₜ) (Pₛ: prog Λₛ) (Φ: value Λₜ -> value Λₛ -> Prop).
+
+  Notation "t '⟨' iₜ '≲' iₛ '⟩' s '{{' Φ '}}'" :=
+    (fsim Wₜ Wₛ Pₜ Pₛ Φ iₜ t iₛ s)
+      (at level 70, iₜ at level 69, iₛ at level 69, no associativity).
+
+  Definition StatePair := (state Λₜ * state Λₛ)%type.
+
+  Notation "t '⦉' iₜ ',' wₜ '≲' iₛ ',' wₛ '⦊' s '{{' Φ '}}'" :=
+    (gsim Wₜ Wₛ (WfOrdTree StatePair) Pₜ Pₛ Φ iₜ wₜ t iₛ wₛ s)
+      (at level 70, iₜ at level 69, iₛ at level 69, no associativity).
+
+  Notation "t '⟪' Rₜ ','  wₜ '≲' Rₛ ',' wₛ '⟫' s '{{' Φ '}}'" :=
+    (ealt_sim Rₜ Rₛ Pₜ Pₛ Φ wₜ t wₛ s)
+      (at level 70, wₜ at level 69, wₛ at level 69, no associativity).
+
+  Lemma gsim_implies_ealt_sim: ∀ iₜ wₜ t iₛ wₛ s,
+    t ⦉ iₜ, wₜ ≲ iₛ, wₛ ⦊ s {{Φ}} ->
+    ∃ Rₜ Rₛ zₜ zₛ, t ⟪ Rₜ, zₜ ≲ Rₛ, zₛ ⟫ s {{Φ}}.
+  Proof.
+    intros iₜ wₜ t iₛ wₛ s Hsim.
+    exists (WfLexProd Wₛ _), (WfLexProd Wₜ _), (iₛ, wₜ), (iₜ, wₛ).
+    revert iₜ wₜ t iₛ wₛ s Hsim.
+    unfold ealt_sim.
+    coinduction R cih.
+    intros iₜ.
+    induction iₜ as [iₜ IHi] using (well_founded_induction wf).
+    intros wₜ t iₛ wₛ s Hsim.
+    induction Hsim as
+      [ iₜ wₜ t iₛ wₛ s Hfin
+      | iₜ wₜ t iₛ wₛ s Hstuck
+      | iₜ wₜ t iₛ iₛ' wₛ s s' wₛ' Hstep Hlt Hsim IHs
+      | iₜ wₜ t iₛ wₛ s Hprogress IHt
+      | iₜ iₜ' wₜ t iₛ iₛ' wₛ s Ht Hs Hsim].
+    - now constructor.
+    - now constructor.
+    - eapply EAltSourceSteps.
+      { eassumption. }
+      { right. eassumption. }
+      apply cih. eassumption.
+    - apply EAltTargetSteps.
+      { assumption. }
+      intros t' Hstep.
+      edestruct (IHt _ Hstep) as (iₜ' & wₜ' & Hlt & Hsim & IH).
+      eexists. eexists. split.
+      { right. eassumption. }
+      apply cih. eassumption.
+    - apply fsim_implies_gsim in Hsim.
+      destruct Hsim as (wₜ' & wₛ' & Hsim).
+      eapply IHi in Hsim; try assumption.
+      clear cih IHi.
+      eapply test.
+      eassumption.
+      + left. now left.
+      + left. now left.
+  Qed.
+End PROOF.
