theories/Simulations/ExplicitSim.v
@@ -1,0 +1,67 @@
+From RSL Require Import Prelude.
+
+From Coinduction Require Import all.
+
+From RSL Require Import Simulations.Commons.
+
+(* Set Mangle Names. *)
+
+Section ESimDef.
+  Context {Λₜ Λₛ: lang}.
+  Context (W: WfRel) (Pₜ: prog Λₜ) (Pₛ: prog Λₛ) (Φ: value Λₜ -> value Λₛ -> Prop).
+
+  Variant esim_lfp' (gfp: W -> state Λₜ -> state Λₛ -> Prop)
+    : W -> state Λₜ -> state Λₛ -> Prop :=
+  | EBothFinal : ∀ i t s,
+    is_final Φ t s -> esim_lfp' gfp i t s
+
+  | ESourceStuck : ∀ i t s,
+    stuck Pₛ s -> esim_lfp' gfp i t s
+
+  | ESourceSteps : ∀ i i' t s s',
+    Pₛ ⊨ s ->> s' ->
+    i' ⊏ i ->
+    gfp i' t s' ->
+    esim_lfp' gfp i t s
+
+  | ETargetSteps : ∀ i t s,
+    can_progress Pₜ t ->
+    (∀ t', Pₜ ⊨ t ->> t' -> ∃ i', i' ⊏ i ∧ gfp i' t' s) ->
+    esim_lfp' gfp i t s
+
+  | EBothSteps : ∀ i t s,
+    can_progress Pₜ t ->
+    (∀ t', Pₜ ⊨ t ->> t' -> ∃ i' s', Pₛ ⊨ s ->> s' ∧ gfp i' t' s') ->
+    esim_lfp' gfp i t s.
+
+  Program Definition esim_lfp : mon (element W -> state Λₜ -> state Λₛ -> Prop) :=
+    {| body := esim_lfp' |}.
+  Next Obligation.
+    intros gfp gfp' Hgfp i t s Hsim.
+    inv Hsim as [ | | | ? ? ? Hprogress Ht |  ? ? ? Hprogress Hboth].
+    - now constructor.
+    - now constructor.
+    - eapply ESourceSteps; eauto.
+      now apply Hgfp.
+    - eapply ETargetSteps; eauto.
+      intros t' Hstep.
+      destruct (Ht _ Hstep) as (i' & ? & ?).
+      exists i'. split; auto.
+      now apply Hgfp.
+    - eapply EBothSteps; eauto.
+      intros t' Hstep.
+      destruct (Hboth _ Hstep) as (i' & s' & ? & ?).
+      exists i', s'. split; auto.
+      now apply Hgfp.
+  Qed.
+
+  Lemma esim_unroll i t s :
+    gfp esim_lfp i t s -> esim_lfp' (gfp esim_lfp) i t s.
+  Proof. apply (gfp_fp esim_lfp). Qed.
+
+  Lemma esim_roll i t s :
+    esim_lfp' (gfp esim_lfp) i t s -> gfp esim_lfp i t s.
+  Proof. apply (gfp_fp esim_lfp). Qed.
+
+  Definition esim  := gfp esim_lfp.
+End ESimDef.
