theories/Simulations/FreeSim.v
@@ -1,0 +1,153 @@
+From RSL Require Import Prelude.
+
+From Coinduction Require Import all.
+
+From RSL Require Import Simulations.Commons.
+
+(* Set Mangle Names. *)
+
+Section FSimDef.
+  Context {Λₜ Λₛ: lang}.
+  Context (Wₜ Wₛ: WfRel).
+  Context (Pₜ: prog Λₜ) (Pₛ: prog Λₛ) (Φ: value Λₜ -> value Λₛ -> Prop).
+
+  Unset Elimination Schemes.
+
+  Inductive fsim_lfp' (gfp: Wₜ -> state Λₜ -> Wₛ -> state Λₛ -> Prop)
+    : Wₜ -> state Λₜ -> Wₛ -> state Λₛ -> Prop :=
+  | FBothFinal : ∀ iₜ t iₛ s,
+    is_final Φ t s -> fsim_lfp' gfp iₜ t iₛ s
+
+  | FSourceStuck : ∀ iₜ t iₛ s,
+    stuck Pₛ s -> fsim_lfp' gfp iₜ t iₛ s
+
+  | FSourceSteps : ∀ iₜ t iₛ iₛ' s s',
+    Pₛ ⊨ s ->> s' ->
+    fsim_lfp' gfp iₜ t iₛ' s' ->
+    fsim_lfp' gfp iₜ t iₛ s
+
+  | FTargetSteps : ∀ iₜ t iₛ s,
+    can_progress Pₜ t ->
+    (∀ t', Pₜ ⊨ t ->> t' -> ∃ iₜ', fsim_lfp' gfp iₜ' t' iₛ s) ->
+    fsim_lfp' gfp iₜ t iₛ s
+
+  | FProgress : ∀ iₜ iₜ' t iₛ iₛ' s,
+    iₜ' ⊏ iₜ ->
+    iₛ' ⊏ iₛ ->
+    gfp iₜ' t iₛ' s ->
+    fsim_lfp' gfp iₜ t iₛ s.
+
+  Set Elimination Schemes.
+
+  Section FSimInd.
+    Variable gfp : Wₜ -> state Λₜ -> Wₛ -> state Λₛ -> Prop.
+    Variable P : Wₜ -> state Λₜ -> Wₛ -> state Λₛ -> Prop.
+
+    Hypothesis HFinal:
+      ∀ iₜ t iₛ s, is_final Φ t s -> P iₜ t iₛ s.
+
+    Hypothesis HStuck:
+      ∀ iₜ t iₛ s, stuck Pₛ s -> P iₜ t iₛ s.
+
+    Hypothesis HSourceSteps:
+      ∀ iₜ t iₛ iₛ' s s',
+      Pₛ ⊨ s ->> s' ->
+      fsim_lfp' gfp iₜ t iₛ' s' ->
+      P iₜ t iₛ' s' ->
+      P iₜ t iₛ s.
+
+    Hypothesis HTargetSteps:
+      ∀ iₜ t iₛ s,
+      can_progress Pₜ t ->
+      (∀ t', Pₜ ⊨ t ->> t' ->
+             ∃ iₜ',
+               fsim_lfp' gfp iₜ' t' iₛ s ∧
+               P iₜ' t' iₛ s) ->
+      P iₜ t iₛ s.
+
+    Hypothesis HProgress:
+      ∀ iₜ iₜ' t iₛ iₛ' s,
+      iₜ' ⊏ iₜ ->
+      iₛ' ⊏ iₛ ->
+      gfp iₜ' t iₛ' s ->
+      P iₜ t iₛ s.
+
+    Lemma fsim_lfp'_ind: ∀ iₜ t iₛ s,
+      fsim_lfp' gfp iₜ t iₛ s -> P iₜ t iₛ s.
+    Proof.
+      fix IH 5. intros iₜ t iₛ s Hsim.
+      destruct Hsim as
+        [ iₜ t iₛ s Hfin
+        | iₜ t iₛ s Hstuck
+        | iₜ t iₛ' iₛ s s' Hstep Hsim
+        | iₜ t iₛ s Hprogress Ht
+        | iₜ iₜ' t iₛ iₛ' s Ht Hs Hgfp ].
+      - apply HFinal. assumption.
+      - apply HStuck. assumption.
+      - eapply HSourceSteps; now eauto.
+      - apply HTargetSteps.
+        { assumption. }
+        intros t' Hstep.
+        destruct (Ht _ Hstep) as (iₜ' & Hsim).
+        exists iₜ'. now auto.
+      - eapply HProgress; now eauto.
+    Qed.
+  End FSimInd.
+
+  Register Scheme fsim_lfp'_ind as ind_nodep for fsim_lfp'.
+
+  Program Definition fsim_lfp : mon (Wₜ -> state Λₜ -> Wₛ -> state Λₛ -> Prop) :=
+    {| body := fsim_lfp' |}.
+  Next Obligation.
+    intros gfp gfp' Hgfp iₜ t iₛ s Hsim.
+    induction Hsim as [ | | | ? ? ? ? Hprogress Ht |  ? ? ? Hprogress Hboth].
+    - econstructor; eassumption.
+    - econstructor; eassumption.
+    - econstructor; eassumption.
+    - apply FTargetSteps; auto. intros ? Hstep.
+      destruct (Ht _ Hstep) as (i & Isim & IH).
+      exists i. auto.
+    - eapply FProgress; try eassumption.
+      apply Hgfp. eassumption.
+  Qed.
+
+  Lemma fsim_unroll iₜ t iₛ s :
+    gfp fsim_lfp iₜ t iₛ s -> fsim_lfp' (gfp fsim_lfp) iₜ t iₛ s.
+  Proof. apply (gfp_fp fsim_lfp). Qed.
+
+  Lemma fsim_roll iₜ t iₛ s :
+    fsim_lfp' (gfp fsim_lfp) iₜ t iₛ s -> gfp fsim_lfp iₜ t iₛ s.
+  Proof. apply (gfp_fp fsim_lfp). Qed.
+
+  Definition fsim  := gfp fsim_lfp.
+
+  Lemma idx_mono: ∀ iₜ iₜ' iₛ iₛ' t s,
+    iₜ' ⊑ iₜ ->
+    iₛ' ⊑ iₛ ->
+    fsim iₜ' t iₛ' s ->
+    fsim iₜ t iₛ s.
+  Proof.
+    unfold fsim at 2.
+    coinduction C CIH.
+    intros iₜ iₜ' iₛ iₛ' t s Ht Hs Hsim.
+    apply fsim_unroll in Hsim.
+    induction Hsim as [ ? t ? s Hfin
+                      | ? t ? s Hstuck
+                      | ? t ? ? s s' Hstep Hsim IH
+                      | ? t ? s Hprog IH
+                      | ? ? t  ? ? s Htt Hss Hsim ]
+      in iₜ, iₜ', iₛ, iₛ', t, s, Ht, Hs, Hsim |- *.
+    - now constructor.
+    - now constructor.
+    - eapply FSourceSteps.
+      { eassumption. }
+      apply IH; assumption || reflexivity.
+    - apply FTargetSteps.
+      { assumption. }
+      intros t' Hstep.
+      destruct (IH _ Hstep) as (iₜ' & Hsim & IHt).
+      eexists. apply IHt; assumption || reflexivity.
+    - admit.
+  Admitted.
+
+End FSimDef.
