theories/Simulations/ImplicitSim.v
@@ -1,0 +1,54 @@
+From RSL Require Import Prelude.
+
+From Coinduction Require Import all.
+
+From RSL Require Import Simulations.Commons.
+
+(* Set Mangle Names. *)
+
+Section ISimDef.
+  Context {Λₜ Λₛ: lang}.
+  Context (Pₜ: prog Λₜ) (Pₛ: prog Λₛ) (Φ: value Λₜ -> value Λₛ -> Prop).
+
+  Inductive isim_lfp'
+    (gfp: state Λₜ -> state Λₛ -> Prop) : state Λₜ -> state Λₛ-> Prop :=
+  | IBothFinal : ∀ t s,
+    is_final Φ t s -> isim_lfp' gfp t s
+
+  | ISourceStuck : ∀ t s,
+    stuck Pₛ s -> isim_lfp' gfp t s
+
+  | ISourceSteps : ∀ t s s',
+    Pₛ ⊨ s ->> s' -> isim_lfp' gfp t s' -> isim_lfp' gfp t s
+
+  | ITargetSteps : ∀ t s,
+    can_progress Pₜ t ->
+    (∀ t', Pₜ ⊨ t ->> t' -> isim_lfp' gfp t' s) ->
+    isim_lfp' gfp t s
+
+  | IBothSteps : ∀ t s,
+    can_progress Pₜ t ->
+    (∀ t', Pₜ ⊨ t ->> t' -> ∃ s', Pₛ ⊨ s ->> s' ∧ gfp t' s') ->
+    isim_lfp' gfp t s.
+
+  Instance isim_lfp'_proper : Proper (leq ==> leq) isim_lfp'.
+  Proof.
+    intros gfp gfp' Hgfp s t H. induction H as [ | | | | ? ? ? H ];
+      try (econstructor; eassumption || now apply Hlfp).
+    apply IBothSteps; eauto. intros t' Hstep.
+    destruct (H _ Hstep) as (? & ? & ?).
+    eexists. split; eassumption || now apply Hgfp.
+  Qed.
+
+  Definition isim_lfp : mon (state Λₜ -> state Λₛ -> Prop) := {| body := isim_lfp' |}.
+
+  Lemma isim_unroll t s :
+    gfp isim_lfp t s -> isim_lfp' (gfp isim_lfp) t s.
+  Proof. apply (gfp_fp isim_lfp). Qed.
+
+  Lemma isim_roll t s :
+    isim_lfp' (gfp isim_lfp) t s -> gfp isim_lfp t s.
+  Proof. apply (gfp_fp isim_lfp). Qed.
+
+  Definition isim := gfp isim_lfp.
+End ISimDef.
