theories/Simulations/Soundness/ExplicitSound.v
@@ -1,0 +1,231 @@
+From RSL Require Import Prelude.
+
+From Stdlib Require Import Classical.
+From Coinduction Require Import all.
+
+From RSL Require Import Simulations.Commons.
+From RSL Require Import Simulations.Behaviors.
+From RSL Require Import Simulations.ExplicitSim.
+
+(* Set Mangle Names. *)
+
+Section ESimSound.
+  Context {Λₜ Λₛ: lang}.
+  Context (W: WfRel) (Pₜ: prog Λₜ) (Pₛ: prog Λₛ).
+
+  Instance behₜ_elem : ElemOf behavior (state Λₜ) := beh Pₜ.
+  Instance behₛ_elem : ElemOf behavior (state Λₛ) := beh Pₛ.
+
+  Notation "a '⊑{' Φ '}' b" :=
+    (behavior_order Φ a b)
+      (at level 70, format "a  '⊑{' Φ '}'  b", no associativity).
+
+  Notation "t '≲' '[' i ']' s '{{' Φ '}}'" :=
+    (esim W Pₜ Pₛ Φ i t s)
+      (at level 70, no associativity).
+
+  Lemma terminating_esim Φ : ∀ i t s vₜ,
+    t ≲[i] s {{ Φ }} ->
+    Terminating vₜ ∈ t ->
+    ∃ b, b ∈ s ∧ Terminating vₜ ⊑{Φ} b.
+  Proof.
+    intros i t s vₜ Hsim Hb.
+    (* t Terminates -> it reduces to a final state *)
+    apply has_terminating_behavior in Hb. destruct Hb as (t' & Hrtc & Hfin).
+    revert i s Hsim.
+    (* Induction on the reduction *)
+    induction Hrtc as [ t | t u t' Ht Hrtc IHt ]; intros i.
+    - (* t is final *)
+      (* Induction on the stuttering index *)
+      induction i as [i IHi] using (well_founded_induction wf).
+      intros s Hsim.
+      (* Induction on the least-fixpoint of the relation *)
+      apply esim_unroll in Hsim.
+      induction Hsim as [ i t s Hfinal
+                        | i t s Hstuck
+                        | i i' t s s' Hs Hlt Hgfp
+                        | i t s Hprogress Ht
+                        | i t s Hprogress Ht ].
+      + (* Both Final *)
+        destruct Hfinal as (? & vₛ & Ht & ? & ?).
+        (* s is final too *)
+        inv Ht. exists (Terminating vₛ). now do 2 constructor.
+      + (* Source Stuck *)
+        exists Undef. split; now constructor.
+      + (* Source Steps, use IH on stuttering index *)
+        destruct (IHi _ Hlt _ Hgfp) as (b & Hbeh & Horder).
+        exists b. split; auto.
+        eapply IsSteping; now eauto.
+      + (* Target Steps -> contradiction *)
+        mixin.
+      + (* Both Steps -> contradiction *)
+        mixin.
+    - (* t steps *)
+      (* Induction on the stuttering index *)
+      induction i as [i IHi] using (well_founded_induction wf).
+      intros s Hsim.
+      (* Induction on the least-fixpoint of the relation *)
+      apply esim_unroll in Hsim.
+      induction Hsim as [ i t s Hfinal
+                        | i t s Hstuck
+                        | i i' t s s' Hs Hlt Hgfp
+                        | i t s Hprogress IH
+                        | i t s Hprogress IH ].
+      + (* Both Final -> contradiction *)
+        destruct Hfinal as (? & ? & ? & ? & ?). mixin.
+      + (* Source Stuck *)
+        exists Undef. split; now constructor.
+      + (* Source Steps, use IH on stuttering index *)
+        destruct (IHi _ Hlt _ Hgfp) as (b & Hbeh & Horder).
+        exists b. split; auto.
+        eapply IsSteping; now eauto.
+      + (* Target Steps, use IH on t *)
+        destruct (IH _ Ht) as (i' & Hlt & Hgfp).
+        apply IHt with i'; now auto.
+      + (* Both Steps, use IH on t *)
+        destruct (IH _ Ht) as (i' & s' & Hs & Hgfp).
+        edestruct IHt as (b & Hbeh & ?); eauto.
+        exists b. split; auto.
+        eapply IsSteping; now eauto.
+  Qed.
+
+  Lemma esim_lfp_progress Φ : ∀ i t s,
+    t ≲[i] s {{ Φ }} ->
+    diverges Pₜ t ->
+    stuck Pₛ s ∨
+      ∃ i' t' s', Pₛ ⊨ s ->> s' ∧ t' ≲[i'] s' {{ Φ }} ∧ diverges Pₜ t'.
+  Proof.
+    intros i.
+    (* Induction on the progress index *)
+    induction i as [i IHi] using (well_founded_induction wf).
+    intros t s Hsim Hdiv.
+    (* Induction on the least-fixpoint of the relation *)
+    apply esim_unroll in Hsim.
+    induction Hsim as [ i t s Hfinal
+                      | i t s Hstuck
+                      | i i' t s s' Hs Hlt Hgfp
+                      | i t s Hprogress IHt
+                      | i t s Hprogress IHt ].
+    - (* Both Final: Contradiction *)
+      destruct Hfinal as (vₜ & vₛ & Ht_fin & Hs_fin & HPhi).
+      apply diverges_unroll in Hdiv. destruct Hdiv as (t' & Ht_step & _).
+      mixin.
+    - (* Source Stuck *)
+      left. exact Hstuck.
+    - (* Source Steps *)
+      right. exists i', t, s'. now auto.
+    - (* Target Steps *)
+      (* t can progress, source waits. Because t diverges, it steps to t' *)
+      apply diverges_unroll in Hdiv. destruct Hdiv as (t' & Ht_step & Hdiv_t').
+      (* Use IHt to lower progress index *)
+      destruct (IHt t' Ht_step) as (i' & Hlt & Hgfp).
+      (* Use IHi on new progress index *)
+      destruct (IHi _ Hlt _ _ Hgfp); now auto.
+    - (* Both Steps *)
+      apply diverges_unroll in Hdiv. destruct Hdiv as (t' & Ht_step & Hdiv_t').
+      (* Use IH on t to make s steps *)
+      destruct (IHt t' Ht_step) as (i' & s' & Hstep & Hgfp).
+      right. exists i', t', s'. now auto.
+  Qed.
+
+  Lemma diverging_esim Φ : ∀ i t s,
+    t ≲[i] s {{ Φ }} ->
+    Diverging ∈ t ->
+    ∃ b, b ∈ s ∧ Diverging ⊑{Φ} b.
+  Proof.
+    intros i t s Hsim Hdiv.
+    (* We see in the future: can s be stuck ? *)
+    destruct (classic (∃ s', Pₛ ⊨ s ->>* s' ∧ stuck Pₛ s')) as [Hstuck | Hnstuck].
+    - (* s can be stuck -> s has Undef behavior *)
+      exists Undef. split; now apply has_undef_behavior || constructor.
+    - (* s is never stuck -> s is diverging *)
+      exists Diverging. split; try constructor.
+      apply has_diverging_behavior in Hdiv.
+      (* We prove by coinduction that s diverges *)
+      unfold diverges.
+      revert i t s Hdiv Hsim Hnstuck. coinduction ξ cih.
+      intros i t s Hdiv Hsim Hnstuck.
+      (* [sim_lfp_progress] give us s' such that s ->> s' *)
+      destruct (esim_lfp_progress _ _ _ _ Hsim Hdiv) as
+        [Hstuck | (i' & t' & s' & Hstep & Hsim' & Hdiv')].
+      + (* s is stuck -> contradiction *)
+        exfalso. apply Hnstuck. exists s. split; auto.
+      + (* s steps *)
+        exists s'. split; auto. eapply cih; eauto.
+        intros (s'' & ? & ? ).
+        apply Hnstuck. exists s''. split; auto.
+        econstructor; now eauto.
+  Qed.
+
+  Lemma undef_esim Φ : ∀ i t s,
+    t ≲[i] s {{ Φ }} ->
+    Undef ∈ t ->
+    Undef ∈ s.
+  Proof.
+    intros i t s Hsim Hb.
+    (* t reach a stuck state. *)
+    apply has_undef_behavior in Hb. destruct Hb as (t' & Hrtc & Hstuck).
+    revert i s Hsim.
+    (* Induction on the reduction *)
+    induction Hrtc as [ t | t u t' Htstep Hrtc IHt ]; intros i.
+    - (* t = t' *)
+      (* Induction on the stuttering index *)
+      induction i as [i IHi] using (well_founded_induction wf).
+      intros s Hsim.
+      (* Induction on the least-fixpoint of the relation *)
+      apply esim_unroll in Hsim.
+      induction Hsim as [ i t s Hfinal
+                        | i t s Hstucks
+                        | i i' t s s' Hs Hlt Hgfp
+                        | i t s Hprogress _
+                        | i t s Hprogress _ ].
+      + (* Both Final -> contradiction *)
+        destruct Hfinal as (? & vₛ & Ht & ? & ?).
+        mixin.
+      + (* Source Stuck -> trivial *)
+        now constructor.
+      + (* Source Steps, use IH on progress index *)
+        eapply IsSteping; eauto.
+        eapply IHi; now eauto.
+      + (* Target Steps -> contradiction *)
+        mixin.
+      + (* Both Steps -> contradiction *)
+        mixin.
+    - (* t steps *)
+      (* Induction on the stuttering index *)
+      induction i as [i IHi] using (well_founded_induction wf).
+      intros s Hsim.
+      (* Induction on the least-fixpoint of the relation *)
+      apply esim_unroll in Hsim.
+      induction Hsim as [ i t s Hfinal
+                        | i t s Hstucks
+                        | i i' t s s' Hs Hlt Hgfp
+                        | i t s Hprogress Ht
+                        | i t s Hprogress Ht ].
+      + (* Both Final -> contradiction *)
+        destruct Hfinal as (? & ? & ? & ? & ?). mixin.
+      + (* Source Stuck -> trivial *)
+        now constructor.
+      + (* Source Steps, use IH on progress index *)
+        eapply IsSteping; eauto.
+        eapply IHi; now eauto.
+      + (* Target Steps, use IH on t *)
+        destruct (Ht _ Htstep) as (i' & _ & Hgfp).
+        apply IHt with i'; now auto.
+      + (* Both Steps, use IH on t *)
+        destruct (Ht _ Htstep) as (i' & s' & Hstep & Hgfp).
+        apply IHt in Hgfp; auto.
+        eapply IsSteping; now eauto.
+  Qed.
+
+  Theorem esim_sound Φ : ∀ i t s,
+    t ≲[i] s {{ Φ }} -> refines Pₜ Pₛ Φ t s.
+  Proof.
+    intros i t s Hsim [] Hb.
+    - eapply terminating_esim; now eauto.
+    - eapply diverging_esim; now eauto.
+    - exists Undef. split.
+      + eapply undef_esim; now eauto.
+      + now constructor.
+  Qed.
+End ESimSound.
