theories/Simulations/Soundness/FreeSound.v
@@ -1,0 +1,240 @@
+From RSL Require Import Prelude.
+
+From Stdlib Require Import Classical.
+From Coinduction Require Import all.
+
+From RSL Require Import Simulations.Commons.
+From RSL Require Import Simulations.Behaviors.
+From RSL Require Import Simulations.FreeSim.
+
+(* Set Mangle Names. *)
+
+Section FSimSound.
+  Context {Λₜ Λₛ: lang}.
+  Context {Wₜ Wₛ: WfRel}.
+  Context (Pₜ: prog Λₜ) (Pₛ: prog Λₛ).
+
+  Instance behₜ_elem : ElemOf behavior (state Λₜ) := beh Pₜ.
+  Instance behₛ_elem : ElemOf behavior (state Λₛ) := beh Pₛ.
+
+  Notation "a '⊑{' Φ '}' b" :=
+    (behavior_order Φ a b)
+      (at level 70, format "a  '⊑{' Φ '}'  b", no associativity).
+
+  Notation "'⟨' t ',' it '⟩' '≲' '⟨' s ',' is '⟩' '{{' Φ '}}'" :=
+    (fsim Wₜ Wₛ Pₜ Pₛ Φ it t is s)
+      (at level 70, no associativity).
+
+  Lemma terminating_fsim Φ : ∀ t iₜ s iₛ vₜ,
+    ⟨t, iₜ⟩ ≲ ⟨s, iₛ⟩ {{ Φ }} ->
+    Terminating vₜ ∈ t ->
+    ∃ b, b ∈ s ∧ Terminating vₜ ⊑{Φ} b.
+  Proof.
+    intros t iₜ s iₛ vₜ Hsim Hb.
+    (* t Terminates -> it reduces to a final state *)
+    apply has_terminating_behavior in Hb. destruct Hb as (t' & Hrtc & Hfin).
+    (* Induction on the reduction *)
+    revert iₜ iₛ s Hsim.
+    induction Hrtc as [ t | t u t' Hstep Hrtc IHrtc ]; intros iₜ.
+    - (* t is final *)
+      (* Induction on the progress index of t *)
+      induction iₜ as [iₜ IHi] using (well_founded_induction wf).
+      intros s iₛ Hsim.
+      (* Induction on the least-fixpoint of the relation *)
+      apply fsim_unroll in Hsim.
+      induction Hsim as [ iₜ t iₛ s Hfinal
+                        | iₜ t iₛ s Hstuck
+                        | iₜ t iₛ iₛ' s s' Hs ? IHs
+                        | iₜ t iₛ s Hprogress IHt
+                        | iₜ iₜ' t iₛ iₛ' s Hprogress ? Hgfp ].
+      + (* Both Final *)
+        destruct Hfinal as (? & vₛ & Ht & ? & ?).
+        (* s is final too *)
+        inv Ht. exists (Terminating vₛ). now do 2 constructor.
+      + (* Source Stuck *)
+        exists Undef. split; now constructor.
+      + (* Source Steps, use IH on s *)
+        destruct (IHs Hfin) as (b & Hbeh & Horder).
+        { intros. edestruct IHi as (b & Hbeh & Horder); now eauto. }
+        exists b. split; auto.
+        eapply IsSteping; now eauto.
+      + (* Target Steps -> contradiction *)
+        mixin.
+      + (* Coind -> use IH on progress index *)
+        eapply IHi; now eauto.
+    - (* t steps *)
+      (* Induction on the progress index of t *)
+      induction iₜ as [iₜ IHi] using (well_founded_induction wf).
+      intros s iₛ Hsim.
+      (* Induction on the least-fixpoint of the relation *)
+      apply fsim_unroll in Hsim.
+      induction Hsim as [ iₜ t iₛ s Hfinal
+                        | iₜ t iₛ s Hstuck
+                        | iₜ t iₛ iₛ' s s' Hs ? IHs
+                        | iₜ t iₛ s Hprogress IHt
+                        | iₜ iₜ' t iₛ iₛ' s Hprogress ? Hgfp ].
+      + (* Both Final -> contradiction *)
+        destruct Hfinal as (? & ? & ? & ? & ?). mixin.
+      + (* Source Stuck *)
+        exists Undef. split; now constructor.
+      + (* Source Steps, use IH on s *)
+        destruct (IHs Hstep) as (b & Hbeh & Horder).
+        { intros. edestruct IHi as (b & Hbeh & Horder); now eauto. }
+        exists b. split; auto.
+        eapply IsSteping; now eauto.
+      + (* Target Steps, use IH on t *)
+        edestruct (IHt _ Hstep) as (iₜ' & Hsim & IH).
+        eapply IHrtc; auto. apply fsim_roll.
+        now apply Hsim.
+      + (* Coinductive case -> use IH on progress index *)
+        edestruct IHi as (b & Hbeh & Horder); now eauto.
+  Qed.
+
+  Lemma fsim_lfp_progress Φ : ∀ t iₜ s iₛ,
+    ⟨t, iₜ⟩ ≲ ⟨s, iₛ⟩ {{ Φ }} ->
+    diverges Pₜ t ->
+    stuck Pₛ s ∨
+      ∃ t' iₜ' s' iₛ',
+        Pₛ ⊨ s ->> s' ∧
+        diverges Pₜ t' ∧
+        ⟨t', iₜ'⟩ ≲ ⟨s', iₛ'⟩ {{ Φ }}.
+  Proof.
+    intros t iₜ s iₛ.
+    (* Induction on the progress index of s *)
+    revert t iₜ.
+    induction iₛ as [iₛ IHi] using (well_founded_induction wf).
+    intros t iₜ Hsim Hdiv.
+    (* Induction on the least-fixpoint of the relation *)
+    apply fsim_unroll in Hsim.
+    induction Hsim as [ iₜ t iₛ s Hfinal
+                      | iₜ t iₛ s Hstuck
+                      | iₜ t iₛ iₛ' s s' Hs ? IHs
+                      | iₜ t iₛ s Hprogress IHt
+                      | iₜ iₜ' t iₛ iₛ' s Hprogress ? Hgfp ].
+    - (* BothFinal: Contradiction *)
+      destruct Hfinal as (vₜ & vₛ & Ht_fin & Hs_fin & HPhi).
+      apply diverges_unroll in Hdiv. destruct Hdiv as (t' & Hstep & _).
+      mixin.
+    - (* SourceStuck *)
+      left. exact Hstuck.
+    - (* Source Steps *)
+      apply fsim_roll in Hsim.
+      right. repeat econstructor; now eauto.
+    - (* Target Steps *)
+      (* t can progress, source waits. Because t diverges, it steps to t' *)
+      apply diverges_unroll in Hdiv. destruct Hdiv as (t' & Hstep & Hdiv').
+      (* Apply the IH for t' *)
+      edestruct (IHt _ Hstep) as (iₜ' & Hsim & IH).
+      edestruct IH as [ Hstuck | (? & ? & s' & iₛ' & Hs' & Hdiv & Hsim')];
+        try eassumption.
+      + now left.
+      + right. repeat econstructor; now eauto.
+    - (* Coinductive case *)
+      edestruct IHi as [Hstuck | (? & ? & s' & ? & Hs' & Hdiv' & Hsim')];
+        try eassumption.
+      + now left.
+      + right. repeat econstructor; now eauto.
+  Qed.
+
+  Lemma diverging_fsim Φ : ∀ t iₜ s iₛ,
+    ⟨t, iₜ⟩ ≲ ⟨s, iₛ⟩ {{ Φ }} ->
+    Diverging ∈ t ->
+    ∃ b, b ∈ s ∧ Diverging ⊑{Φ} b.
+  Proof.
+    intros t iₜ s iₛ Hsim Hdiv.
+    (* We see in the future: can s be stuck ? *)
+    destruct (classic (∃ s', Pₛ ⊨ s ->>* s' ∧ stuck Pₛ s')) as [Hstuck | Hnstuck].
+    - (* s can be stuck -> s has Undef behavior *)
+      exists Undef. split; now apply has_undef_behavior || constructor.
+    - (* s is never stuck -> s is diverging *)
+      exists Diverging. split; try constructor.
+      apply has_diverging_behavior in Hdiv.
+      (* We prove by coinduction that s diverges *)
+      unfold diverges.
+      revert t iₜ s iₛ Hdiv Hsim Hnstuck.
+      coinduction R cih.
+      intros t iₜ s iₛ Hdiv Hsim Hnstuck.
+      (* [sim_lfp_progress] give us s' such that s ->> s' *)
+      destruct (fsim_lfp_progress _ _ _ _ _ Hsim Hdiv) as
+        [Hstuck | (? & iₜ' & s' & iₛ' & Hs' & ? & ?)].
+      + (* s is stuck -> contradiction *)
+        exfalso. apply Hnstuck. exists s. split; eauto.
+      + (* s steps *)
+        exists s'. split; auto. eapply cih; eauto.
+        intros (s'' & ? & ? ).
+        apply Hnstuck. exists s''. split; auto.
+        econstructor; now eauto.
+  Qed.
+
+  Lemma undef_fsim Φ : ∀ t iₜ s iₛ,
+    ⟨t, iₜ⟩ ≲ ⟨s, iₛ⟩ {{ Φ }} ->
+    Undef ∈ t ->
+    Undef ∈ s.
+  Proof.
+    intros t iₜ s iₛ Hsim Hb.
+    (* t reach a stuck state. *)
+    apply has_undef_behavior in Hb. destruct Hb as (t' & Hrtc & Hstuck).
+    (* Induction on the reduction *)
+    revert iₜ iₛ s Hsim.
+    induction Hrtc as [ t | t u t' Hstep Hrtc IHrtc ]; intros iₜ.
+    - (* t = t' *)
+      (* Induction on the progress index of t *)
+      induction iₜ as [iₜ IHi] using (well_founded_induction wf).
+      intros s iₛ Hsim.
+      (* Induction on the least-fixpoint of the relation *)
+      apply fsim_unroll in Hsim.
+      induction Hsim as [ iₜ t iₛ s Hfinal
+                        | iₜ t iₛ s Hsstuck
+                        | iₜ t iₛ iₛ' s s' Hs ? IHs
+                        | iₜ t iₛ s Hprogress IHt
+                        | iₜ iₜ' t iₛ iₛ' s Hprogress ? Hgfp ].
+      + (* Both Final -> contradiction *)
+        destruct Hfinal as (? & vₛ & Ht & ? & ?).
+        mixin.
+      + (* Source Stuck -> trivial *)
+        now constructor.
+      + (* Source Steps, use IH on s *)
+        eapply IsSteping; eauto.
+        now apply IHs.
+      + (* Target Steps -> contradiction *)
+        mixin.
+      + (* Coinductive case, use IH on progress index *)
+        eapply IHi; now eauto.
+    - (* t steps *)
+      (* Induction on the progress index of t *)
+      induction iₜ as [iₜ IHi] using (well_founded_induction wf).
+      intros s iₛ Hsim.
+      (* Induction on the least-fixpoint of the relation *)
+      apply fsim_unroll in Hsim.
+      induction Hsim as [ iₜ t iₛ s Hfinal
+                        | iₜ t iₛ s Hsstuck
+                        | iₜ t iₛ iₛ' s s' Hs ? IHs
+                        | iₜ t iₛ s Hprogress IHt
+                        | iₜ iₜ' t iₛ iₛ' s Hprogress ? Hgfp ].
+      + (* Both Final -> contradiction *)
+        destruct Hfinal as (? & ? & ? & ? & ?). mixin.
+      + (* Source Stuck -> trivial *)
+        now constructor.
+      + (* Source Steps, use IH on s *)
+        eapply IsSteping; eauto.
+        apply IHs; auto.
+      + (* Target Steps, use IH on t *)
+        edestruct (IHt _ Hstep) as (iₜ' & Hsim & IH).
+        eapply IHrtc; eauto.
+        apply fsim_roll.
+        now apply Hsim.
+      + (* Both Steps, use IH on t *)
+        eapply IHi; now eauto.
+  Qed.
+
+  Theorem fsim_sound Φ : ∀ t iₜ s iₛ,
+    ⟨t, iₜ⟩ ≲ ⟨s, iₛ⟩ {{ Φ }} -> refines Pₜ Pₛ Φ t s.
+  Proof.
+    intros t iₜ s iₛ Hsim [] Hb.
+    - eapply terminating_fsim; now eauto.
+    - eapply diverging_fsim; now eauto.
+    - exists Undef. split.
+      + eapply undef_fsim; now eauto.
+      + now constructor.
+  Qed.
+End FSimSound.
